spec/abstract/ARM/ArchVMAttributes_A.thy
@@ -1,0 +1,52 @@
+(*
+ * Copyright 2014, General Dynamics C4 Systems
+ *
+ * SPDX-License-Identifier: GPL-2.0-only
+ *)
+
+(* Definition of architecture-dependent VM attributes. *)
+
+theory ArchVMAttributes_A
+imports
+  ExecSpec.MachineExports
+begin
+
+context Arch begin global_naming ARM_A
+
+(* Union of attributes and non-seL4 rights that the kernel uses on pages and page tables,
+   including kernel-only attributes. Not all are reachable via attribs_from_word. *)
+datatype vm_attribute = ParityEnabled | PageCacheable | Global | XNever
+type_synonym vm_attributes = "vm_attribute set"
+
+type_synonym arch_raw_vmattrs = word32
+
+definition
+  attribs_from_word :: "word32 \<Rightarrow> vm_attributes" where
+  "attribs_from_word w \<equiv>
+    let V = (if w !!0 then {PageCacheable} else {});
+      V' = (if w!!1 then insert ParityEnabled V else V)
+    in if w!!2 then insert XNever V' else V'"
+
+definition
+  attribs_to_word :: "vm_attributes \<Rightarrow> word32" where
+  "attribs_to_word attribs \<equiv>
+    let V = (if PageCacheable \<in> attribs then 1 else 0);
+      V' = (if ParityEnabled \<in> attribs then V + 2 else V)
+    in if XNever \<in> attribs then V' + 4 else V' "
+
+definition
+  validate_vm_attributes :: "word32 \<Rightarrow> vmpage_size \<Rightarrow> word32"  where
+  "validate_vm_attributes attr sz \<equiv> case sz of
+    ARM.ARMSmallPage \<Rightarrow> attribs_to_word (attribs_from_word attr - {Global, ParityEnabled})
+  | ARM.ARMLargePage \<Rightarrow> attribs_to_word (attribs_from_word attr - {Global, ParityEnabled})
+  | ARM.ARMSection \<Rightarrow> attribs_to_word (attribs_from_word attr - {Global})
+  | ARM.ARMSuperSection \<Rightarrow> attribs_to_word (attribs_from_word attr - {Global})"
+
+definition
+  validate_pt_vm_attributes :: "word32 \<Rightarrow> word32"  where
+  "validate_pt_vm_attributes attr \<equiv> attribs_to_word (attribs_from_word attr \<inter> {ParityEnabled})"
+
+definition default_vmattrs :: "word32" where "default_vmattrs \<equiv> 3"
+
+end
+end
