spec/abstract/VMAttributes_A.thy
@@ -1,0 +1,28 @@
+(*
+ * Copyright 2019, Data61, CSIRO (ABN 41 687 119 230)
+ *
+ * SPDX-License-Identifier: GPL-2.0-only
+ *)
+
+(* Abstract model of VM attributes. *)
+
+theory VMAttributes_A
+imports
+  ArchVMAttributes_A
+begin
+
+arch_requalify_types (A)
+  vm_attribute arch_raw_vmattrs
+
+arch_requalify_consts (A)
+  attribs_from_word
+  attribs_to_word
+  validate_vm_attributes
+  validate_pt_vm_attributes
+  default_vmattrs
+
+arch_requalify_facts (A)
+  validate_vm_attributes_def
+  validate_pt_vm_attributes_def
+
+end
